x86/AsmDummyFrame.v
@@ -1,0 +1,106 @@
+Require Import Smallstep.
+Require Import Machregs.
+Require Import Asm.
+Require Import Integers.
+Require Import List.
+Require Import ZArith.
+Require Import Memtype.
+Require Import Memory.
+Require Import Archi.
+Require Import Coqlib.
+Require Import AST.
+Require Import Globalenvs.
+Require Import Events.
+Require Import Values.
+Require Import Conventions1.
+Require Import AsmFacts.
+
+
+Section WITHEXTERNALCALLS.
+Context `{external_calls_prf: ExternalCalls}.
+
+Variable init_sp: val.
+
+
+Existing Instance mem_accessors_default.
+
+Section RELSEM.
+
+
+  Notation "'do' X <- A ; B" := (match A with Some X => B | None => Stuck end)
+                                  (at level 200, X ident, A at level 100, B at level 200).
+
+  Notation "'do' X , Y <- A ; B" := (match A with Some (X, Y) => B | None => Stuck end)
+                                     (at level 200, X ident, Y ident, A at level 100, B at level 200).
+
+  Notation "'do' X , Y , Z <- A ; B" := (match A with Some (X, Y, Z) => B | None => Stuck end)
+                                         (at level 200, X ident, Y ident, Z ident, A at level 100, B at level 200).
+
+  Notation " 'check' A ; B" := (if A then B else Stuck)
+                                 (at level 200, A at level 100, B at level 200).
+
+
+
+  Definition exec_instr {F V} (ge: Genv.t F V) (f: function) (i: instruction) (rs: regset) (m: mem) : outcome :=
+    match i with
+      Pfreeframe sz ofs_ra =>
+      do ra <- Mem.loadv Mptr m (Val.offset_ptr rs#RSP ofs_ra);
+        match rs#RSP with
+        | Vptr stk ofs =>
+          check (check_top_frame m (Some stk) sz);
+            do m' <- Mem.free m stk 0 sz;
+            check (check_init_sp_in_stack init_sp m');
+            do m' <- Mem.record_stack_blocks m (Build_frame_adt nil 0 (list_norepet_nil _) (Zle_refl _));
+            Next (nextinstr (rs#RSP <-
+                               (match parent_pointer m with
+                                | None => init_sp
+                                | Some (sp,_) => Vptr sp Ptrofs.zero
+                                end) #RA <- ra)) m'
+        | _ => Stuck
+        end
+    | _ => Asm.exec_instr init_sp ge f i rs m
+    end.
+
+  Inductive step (ge: genv) : state -> trace -> state -> Prop :=
+  | exec_step_internal:
+      forall b ofs f i rs m rs' m',
+        rs PC = Vptr b ofs ->
+        Genv.find_funct_ptr ge b = Some (Internal f) ->
+        find_instr (Ptrofs.unsigned ofs) (fn_code f) = Some i ->
+        exec_instr ge f i rs m = Next rs' m' ->
+        step ge (State rs m) E0 (State rs' m')
+  | exec_step_builtin:
+      forall b ofs f ef args res rs m vargs t vres rs' m' m'',
+        rs PC = Vptr b ofs ->
+        Genv.find_funct_ptr ge b = Some (Internal f) ->
+        find_instr (Ptrofs.unsigned ofs) f.(fn_code) = Some (Pbuiltin ef args res) ->
+        eval_builtin_args ge rs (rs RSP) m args vargs ->
+        external_call ef ge vargs (Mem.push_new_stage m) t vres m' ->
+        Mem.unrecord_stack_block m' = Some m'' ->
+        forall BUILTIN_ENABLED: builtin_enabled ef,
+          no_rsp_builtin_preg res ->
+          rs' = nextinstr_nf
+                  (set_res res vres
+                           (undef_regs (map preg_of (destroyed_by_builtin ef)) rs)) ->
+          step ge (State rs m) t (State rs' m'')
+  | exec_step_external:
+      forall b ef args res rs m t rs' m' m'',
+        rs PC = Vptr b Ptrofs.zero ->
+        Genv.find_funct_ptr ge b = Some (External ef) ->
+        extcall_arguments rs m (ef_sig ef) args ->
+        forall (SP_TYPE: Val.has_type (rs RSP) Tptr)
+          (RA_TYPE: Val.has_type (rs RA) Tptr)
+          (SP_NOT_VUNDEF: rs RSP <> Vundef)
+          (RA_NOT_VUNDEF: rs RA <> Vundef),
+          external_call ef ge args m t res m' ->
+          Mem.unrecord_stack_block m' = Some m'' ->
+          no_rsp_pair (loc_external_result (ef_sig ef)) ->
+          rs' = (set_pair (loc_external_result (ef_sig ef)) res (undef_regs (CR ZF :: CR CF :: CR PF :: CR SF :: CR OF :: nil) (undef_regs (map preg_of destroyed_at_call) rs))) #PC <- (rs RA) #RA <- Vundef ->
+          step ge (State rs m) t (State rs' m'').
+
+End RELSEM.
+
+Definition semantics (p: Asm.program) :=
+  Semantics step (initial_state p) final_state (Genv.globalenv p).
+
+End WITHEXTERNALCALLS.
