x86/AsmDummyFrameproof.v
@@ -1,0 +1,174 @@
+Require Import Smallstep.
+Require Import Machregs.
+Require Import Asm.
+Require Import Integers.
+Require Import List.
+Require Import ZArith.
+Require Import Memtype.
+Require Import Memory.
+Require Import Archi.
+Require Import Coqlib.
+Require Import AST.
+Require Import Globalenvs.
+Require Import Events.
+Require Import Values.
+Require Import Conventions1.
+Require Import AsmFacts.
+Require Import AsmDummyFrame.
+
+Section WITHEXTERNALCALLS.
+Context `{external_calls_prf: ExternalCalls}.
+
+Variable init_sp: val.
+Existing Instance mem_accessors_default.
+
+Context `{injperm: InjectPerm}.
+
+Inductive match_states: state -> state -> Prop :=
+| match_states_intro:
+    forall rs1 rs2 m1 m2
+      (MEXT: Mem.extends m1 m2)
+      (REGS: forall r, Val.lessdef (rs1 r) (rs2 r) ),
+      match_states (State rs1 m1) (State rs2 m2).
+
+Variable prog: Asm.program.
+
+Let ge := Genv.globalenv prog.
+
+Lemma mull_lessdef:
+  forall v1 v2 v3 v4,
+    Val.lessdef v1 v3 -> Val.lessdef v2 v4 ->
+    Val.lessdef (Val.mull v1 v2) (Val.mull v3 v4).
+Proof.
+  inversion 1; inversion 1; subst; auto. unfold Val.mull.
+  destr; auto.
+Qed.
+
+Lemma mul_lessdef:
+  forall v1 v2 v3 v4,
+    Val.lessdef v1 v3 -> Val.lessdef v2 v4 ->
+    Val.lessdef (Val.mul v1 v2) (Val.mul v3 v4).
+Proof.
+  inversion 1; inversion 1; subst; auto. unfold Val.mul.
+  destr; auto.
+Qed.
+
+Lemma eval_addrmode_extends:
+  forall rs1 rs2 a,
+    (forall r, Val.lessdef (rs1 r) (rs2 r)) ->
+    Val.lessdef (eval_addrmode ge a rs1) (eval_addrmode ge a rs2).
+Proof.
+  unfold eval_addrmode. intros.
+  destr.
+  unfold eval_addrmode64.
+  destr. apply Val.addl_lessdef. destr; auto.
+  apply Val.addl_lessdef. repeat destr; auto.
+  apply mull_lessdef; auto. auto.
+  unfold eval_addrmode32.
+  destr. apply Val.add_lessdef. destr; auto.
+  apply Val.add_lessdef. repeat destr; auto.
+  apply mul_lessdef; auto. auto.
+Qed.
+
+Lemma exec_load_extends:
+  forall m1 m2 chunk a rs1 rs2 r rs1' m1',
+    match_states (State rs1 m1) (State rs2 m2) ->
+    exec_load ge chunk m1 a rs1 r = Next rs1' m1' ->
+    exists rs2' m2',
+      exec_load ge chunk m2 a rs2 r = Next rs2' m2'
+      /\ match_states (State rs1' m1') (State rs2' m2').
+Proof.
+  intros m1 m2 chunk a rs1 rs2 r rs1' m1' MS EL.
+  unfold exec_load in EL. destr_in EL. inv EL. inv MS.
+  generalize (eval_addrmode_extends _ _ a REGS). intro ADDR.
+  edestruct Mem.loadv_extends as (v2 & LOADV & LD). eauto. eauto. apply ADDR.
+  unfold exec_load. rewrite LOADV. do 2 eexists; split; eauto.
+  constructor; auto.
+  unfold nextinstr_nf. simpl.
+  intros. setoid_rewrite Pregmap.gsspec. destr.
+  apply Val.offset_ptr_lessdef.
+  setoid_rewrite Pregmap.gsspec. destr; eauto.
+  intros. setoid_rewrite Pregmap.gsspec. destr. auto.
+  repeat (setoid_rewrite Pregmap.gsspec; destr; eauto).
+Qed.
+
+Lemma is_freeframe i : {exists sz ora, i = Pfreeframe sz ora} + {forall sz ora, i <> Pfreeframe sz ora}.
+Proof.
+  destruct i; try (right; inversion 1; fail).
+  left; eauto.
+Qed.
+
+Lemma exec_instr_step:
+  forall rs1 m1 rs2 m2,
+    match_states (State rs1 m1) (State rs2 m2) ->
+    forall f i rs1' m1',
+      Asm.exec_instr init_sp ge f i rs1 m1 = Next rs1' m1' ->
+      exists rs2' m2',
+        AsmDummyFrame.exec_instr init_sp ge f i rs2 m2 = Next rs2' m2' /\
+        match_states (State rs1' m1') (State rs2' m2').
+Proof.
+  intros rs1 m1 rs2 m2 MS f i rs1' m1' EI.
+  destruct (is_freeframe i).
+  destruct e as (sz & ora & EQ). subst.
+  - simpl in *. repeat (destr_in EI; [idtac]). inv EI.
+    inv MS.
+    edestruct Mem.loadv_extends as (v' & LOAD & LD); eauto.
+    generalize (REGS RSP). rewrite Heqv0. inversion 1; subst.
+    rewrite LOAD.
+
+    edestruct (exec_load_extends) as (rs2' & m2' & LOADV & MS'); eauto.
+    inv MS.
+
+  destruct i; simpl in *; inv EI; inv MS; try (do 2 eexists; split; eauto; [idtac]); try (constructor; auto).
+  
+
+
+  - constructor; auto. intros. rewrite H4. unfold nextinstr.
+    repeat (setoid_rewrite Pregmap.gsspec; try destr; try setoid_rewrite H4); auto.
+  - constructor; auto. intros. unfold nextinstr_nf.
+    repeat (setoid_rewrite Pregmap.gsspec; try destr; try setoid_rewrite H4); auto.
+  - 
+Qed.
+
+  Inductive step (ge: genv) : state -> trace -> state -> Prop :=
+  | exec_step_internal:
+      forall b ofs f i rs m rs' m',
+        rs PC = Vptr b ofs ->
+        Genv.find_funct_ptr ge b = Some (Internal f) ->
+        find_instr (Ptrofs.unsigned ofs) (fn_code f) = Some i ->
+        exec_instr ge f i rs m = Next rs' m' ->
+        step ge (State rs m) E0 (State rs' m')
+  | exec_step_builtin:
+      forall b ofs f ef args res rs m vargs t vres rs' m' m'',
+        rs PC = Vptr b ofs ->
+        Genv.find_funct_ptr ge b = Some (Internal f) ->
+        find_instr (Ptrofs.unsigned ofs) f.(fn_code) = Some (Pbuiltin ef args res) ->
+        eval_builtin_args ge rs (rs RSP) m args vargs ->
+        external_call ef ge vargs (Mem.push_new_stage m) t vres m' ->
+        Mem.unrecord_stack_block m' = Some m'' ->
+        forall BUILTIN_ENABLED: builtin_enabled ef,
+          no_rsp_builtin_preg res ->
+          rs' = nextinstr_nf
+                  (set_res res vres
+                           (undef_regs (map preg_of (destroyed_by_builtin ef)) rs)) ->
+          step ge (State rs m) t (State rs' m'')
+  | exec_step_external:
+      forall b ef args res rs m t rs' m' m'',
+        rs PC = Vptr b Ptrofs.zero ->
+        Genv.find_funct_ptr ge b = Some (External ef) ->
+        extcall_arguments rs m (ef_sig ef) args ->
+        forall (SP_TYPE: Val.has_type (rs RSP) Tptr)
+          (RA_TYPE: Val.has_type (rs RA) Tptr)
+          (SP_NOT_VUNDEF: rs RSP <> Vundef)
+          (RA_NOT_VUNDEF: rs RA <> Vundef),
+          external_call ef ge args m t res m' ->
+          Mem.unrecord_stack_block m' = Some m'' ->
+          no_rsp_pair (loc_external_result (ef_sig ef)) ->
+          rs' = (set_pair (loc_external_result (ef_sig ef)) res (undef_regs (CR ZF :: CR CF :: CR PF :: CR SF :: CR OF :: nil) (undef_regs (map preg_of destroyed_at_call) rs))) #PC <- (rs RA) #RA <- Vundef ->
+          step ge (State rs m) t (State rs' m'').
+
+End RELSEM.
+
+Definition semantics (p: Asm.program) :=
+  Semantics step (initial_state p) final_state (Genv.globalenv p).
+
